theories/lang/notation.v
@@ -93,13 +93,12 @@ Notation "withcont: k1 : e1 cont: k2 xl := e2" :=
   ((Lam (@cons binder k1%binder nil) e1%E) [Rec k2%binder ((fun _ : eq k1%binder k2%binder => xl%binder) eq_refl) e2%E])
   (only parsing, at level 151, k1, k2, xl at level 1, e2 at level 150) : expr_scope.
 
-Definition call_def (f: expr) (args: list expr) (k: expr) : expr :=
-  (f ((λ: ["_r"], Skip ;; k ["_r"]) :: args))%E.
-Notation "call: f args → k" := (call_def f%E args%E k%E)
+Notation "call: f args → k" :=
+  (App f%E ((λ: [BNamed "_r"], Seq Skip (App k%E [Var "_r"]))%E :: args%E))
   (at level 102, f, args, k at level 1) : expr_scope.
-Definition letcall_def (x: binder) (f: expr) (args: list expr) (e: expr) : expr :=
-  (letcont: "_k" [ x ] := e in call: f args → "_k")%E.
-Notation "letcall: x := f args 'in' e" := (letcall_def x%binder f%E args%E e%E)
+Notation "letcall: x := f args 'in' e" :=
+  (letcont: (BNamed "_k") (@cons binder x%binder nil) := e%E in
+    call: f%E args%E → (Var "_k"))%E
   (at level 102, x, f, args at level 1, e at level 150) : expr_scope.
 
 (* These notations unfortunately do not print.  Also, I don't think
