theories/typing/cont.v
@@ -34,12 +34,12 @@ Section typing.
     rewrite papply_app papp_sepl papp_sepr. case=> Imp ?. by apply Imp.
   Qed.
 
-  Lemma type_cont {𝔄l 𝔅l ℭ} (T: _ 𝔄l) kb bl ec e L' (T': _ → _ 𝔅l)
+  Lemma type_cont {𝔄l 𝔅l ℭ} bl (T': _ → _ 𝔅l) L' (T: _ 𝔄l) kb ec e
     trk tr E L (C: cctx ℭ) :
     Closed (kb :b: bl +b+ []) ec → Closed (kb :b: []) e →
-    (∀k, typed_body E L (k ◁cont{L', T'} trk :: C) T (subst' kb k e) tr) -∗
-    □(∀k (vl: vec val (length bl)), typed_body E L' (k ◁cont{L', T'} trk :: C)
-      (T' vl) (subst' kb k $ subst_v bl vl ec) trk) -∗
+    (∀k: val, typed_body E L (k ◁cont{L', T'} trk :: C) T (subst' kb k e) tr) -∗
+    □(∀(k: val) (vl: vec val (length bl)), typed_body E L'
+      (k ◁cont{L', T'} trk :: C) (T' vl) (subst' kb k $ subst_v bl vl ec) trk) -∗
     typed_body E L C T (letcont: kb bl := ec in e) tr.
   Proof.
     iIntros (??) "e #ec %%% #LFT #TIME #PROPH #UNIQ #E Na L C T Obs".
@@ -50,11 +50,11 @@ Section typing.
     iApply ("ec" with "LFT TIME PROPH UNIQ E Na L' [C] T' Obs"). by iApply "IH".
   Qed.
 
-  Lemma type_cont_norec {𝔄l 𝔅l ℭ} (T: _ 𝔄l) kb bl ec e L' (T': _ → _ 𝔅l)
+  Lemma type_cont_norec {𝔄l 𝔅l ℭ} bl (T': _ → _ 𝔅l) L' (T: _ 𝔄l) kb ec e
     trk tr E L (C: cctx ℭ) :
     Closed (kb :b: bl +b+ []) ec → Closed (kb :b: []) e →
-    (∀k, typed_body E L (k ◁cont{L', T'} trk :: C) T (subst' kb k e) tr) -∗
-    (∀k (vl: vec val (length bl)),
+    (∀k: val, typed_body E L (k ◁cont{L', T'} trk :: C) T (subst' kb k e) tr) -∗
+    (∀(k: val) (vl: vec val (length bl)),
       typed_body E L' C (T' vl) (subst' kb k $ subst_v bl vl ec) trk) -∗
     typed_body E L C T (letcont: kb bl := ec in e) tr.
   Proof.
